Sets/Sets.dfy
@@ -13,31 +13,16 @@ module Sets {
   }
 
   /**
-   * If x is a proper subset of y, then the cardinality of x is less than
-   * the cardinality of y.
-   */
-  lemma lemma_proper_subset_cardinality<T>(x: set<T>, y: set<T>)
-    requires x < y
-    ensures |x| < |y|
-    decreases x, y
-  {
-    if x != {} {
-      var e :| e in x;
-      lemma_proper_subset_cardinality(x - {e}, y - {e});
-    }
-  }
-
-  /**
    * If x is a subset of y, then the cardinality of x is less than or equal to
    * the cardinality of y.
    */
   lemma lemma_subset_cardinality<T>(x: set<T>, y: set<T>)
     ensures x < y ==> |x| < |y|
-    ensures x == y ==> |x| == |y|
+    ensures x <= y ==> |x| <= |y|
   {
-    if x < y {
-      lemma_proper_subset_cardinality(x, y);
-    } else if x == y {
+    if x != {} {
+      var e :| e in x;
+      lemma_subset_cardinality(x - {e}, y - {e});
     }
   }
 
@@ -61,7 +46,7 @@ module Sets {
   /**
    * A singleton set has a cardinality of 1.
    */
-  lemma lemma_singleton_set_cardinality<T>(x: set<T>, e: T)
+  lemma lemma_singleton_cardinality<T>(x: set<T>, e: T)
     requires x == {e}
     ensures |x| == 1
   {
@@ -70,17 +55,17 @@ module Sets {
   /**
    * Elements in a singleton set are equal to each other.
    */
-  lemma lemma_singleton_set_equality<T>(foo: set<T>, x: T, y: T)
-    requires |foo| == 1
-    requires x in foo
-    requires y in foo
+  lemma lemma_singleton_equality<T>(s: set<T>, x: T, y: T)
+    requires |s| == 1
+    requires x in s
+    requires y in s
     ensures x == y
   {
     if x != y {
-      assert {x} < foo;
-      lemma_subset_cardinality({x}, foo);
-      assert |{x}| < |foo|;
-      assert |foo| > 1;
+      assert {x} < s;
+      lemma_subset_cardinality({x}, s);
+      assert |{x}| < |s|;
+      assert |s| > 1;
       assert false;
     }
   }
@@ -89,49 +74,35 @@ module Sets {
    * If an injective function is applied to each element of a set to construct
    * another set, the two sets have the same cardinality. 
    */
-  lemma lemma_map_set_to_set_cardinality<X, Y>(xs: set<X>, ys: set<Y>, f: X-->Y)
+  lemma lemma_apply_cardinality<X(!new), Y>(xs: set<X>, ys: set<Y>, f: X-->Y)
     requires forall x :: f.requires(x)
     requires Math.injective(f)
     requires forall x :: x in xs <==> f(x) in ys
     requires forall y :: y in ys ==> exists x :: x in xs && y == f(x)
     ensures |xs| == |ys|
-    decreases xs, ys
   {
     if xs != {}
     {
       var x :| x in xs;
       var xs' := xs - {x};
       var ys' := ys - {f(x)};
-      lemma_map_set_to_set_cardinality(xs', ys', f);
+      lemma_apply_cardinality(xs', ys', f);
     }
   }
 
   /**
    * Apply an injective function to each element of a set.
    */
-  function method {:opaque} map_set_to_set<X(!new), Y>(xs: set<X>, f: X-->Y): set<Y>
+  function method {:opaque} apply<X(!new), Y>(xs: set<X>, f: X-->Y): set<Y>
     reads f.reads
     requires forall x :: f.requires(x)
     requires Math.injective(f)
-    ensures forall x :: x in xs <==> f(x) in map_set_to_set(xs, f)
-    ensures |xs| == |map_set_to_set(xs, f)|
+    ensures forall x :: x in xs <==> f(x) in apply(xs, f)
+    ensures |xs| == |apply(xs, f)|
   {
     var ys := set x | x in xs :: f(x); 
-    lemma_map_set_to_set_cardinality(xs, ys, f);
+    lemma_apply_cardinality(xs, ys, f);
     ys
-  }
-
-  /**
-   * Apply an injective function to each element of a sequence.
-   */
-  function method {:opaque} map_seq_to_set<X(!new), Y>(xs: seq<X>, f: X-->Y): set<Y>
-    reads f.reads
-    requires forall x :: f.requires(x)
-    requires Math.injective(f)
-    ensures forall x :: x in xs <==> f(x) in map_seq_to_set(xs, f)
-    decreases xs
-  {
-    if |xs| == 0 then {} else map_seq_to_set(xs[1..], f) + {f(xs[0])}
   }
 
   /**
@@ -158,7 +129,7 @@ module Sets {
    * Construct a set using elements of another set for which a function returns
    * true.
    */
-  function method {:opaque} filter<X(!new)>(xs: set<X>, f: X~>bool): set<X>
+  function {:opaque} filter<X(!new)>(xs: set<X>, f: X~>bool): set<X>
     reads f.reads
     requires forall x :: x in xs ==> f.requires(x)
     ensures forall y :: y in filter(xs, f) <==> y in xs && f(y)
@@ -170,14 +141,12 @@ module Sets {
   }
 
   /**
-   * The cardinality of a union of two sets greater than the cardinality of
-   * either individual set.
+   * The cardinality of a union of two sets is greater than or equal to the
+   * cardinality of either individual set.
    */
-  lemma lemma_union_cardinality<X>(xs: set<X>, ys: set<X>, us: set<X>)
-    requires us == xs + ys
-    ensures |us| >= |xs|
-    ensures |us| >= |ys|
-    decreases ys
+  lemma lemma_union_cardinality<X>(xs: set<X>, ys: set<X>)
+    ensures |xs + ys| >= |xs|
+    ensures |xs + ys| >= |ys|
   {
     if ys == {} {
     } else {
@@ -185,48 +154,20 @@ module Sets {
       if y in xs {
         var xr := xs - {y};
         var yr := ys - {y};
-        var ur := us - {y};
-        lemma_union_cardinality(xr, yr, ur);
+        assert xr + yr == xs + ys - {y};
+        lemma_union_cardinality(xr, yr);
       } else {
-        var ur := us - {y};
         var yr := ys - {y};
-        lemma_union_cardinality(xs, yr, ur);
+        assert xs + yr == xs + ys - {y};
+        lemma_union_cardinality(xs, yr);
       }
-    }
-  }
-
-  /**
-   * Construct a set with all integers in the range [0, n).
-   */
-  function set_range_zero_bound(n: int): set<int>
-    requires n >= 0
-    ensures forall i :: 0 <= i < n <==> i in set_range_zero_bound(n)
-    ensures |set_range_zero_bound(n)| == n
-    decreases n
-  {
-    if n == 0 then {} else {n - 1} + set_range_zero_bound(n - 1)
-  }
-
-  /**
-   * If a set contains all integers in the range [0, n), then its cardinality is
-   * n.
-   */
-  lemma {:induction n} lemma_set_range_cardinality(n: int)
-    requires n >= 0
-    ensures |set_range_zero_bound(n)| == n
-    decreases n
-  {
-    if n == 0 {
-    } else {
-      lemma_set_range_cardinality(n - 1);
-      assert set_range_zero_bound(n) == set_range_zero_bound(n - 1) + {n - 1};
     }
   }
 
   /**
    * Construct a set with all integers in the range [a, b).
    */
-  function method set_range(a: int, b: int): set<int>
+  function method {:opaque} set_range(a: int, b: int): set<int>
     requires a <= b
     ensures forall i :: a <= i < b <==> i
             in set_range(a, b)
@@ -234,6 +175,17 @@ module Sets {
     decreases b - a
   {
     if a == b then {} else {a} + set_range(a + 1, b)
+  }
+
+  /**
+   * Construct a set with all integers in the range [0, n).
+   */
+  function method {:opaque} set_range_zero_bound(n: int): set<int>
+    requires n >= 0
+    ensures forall i :: 0 <= i < n <==> i in set_range_zero_bound(n)
+    ensures |set_range_zero_bound(n)| == n
+  {
+    set_range(0, n)
   }
 
   /**
